\documentclass[12pt,a4paper]{article}
\usepackage{graphicx}
\usepackage{amsmath}
\usepackage{bm}
\usepackage{interval}
\usepackage{amssymb}
\usepackage[letterpaper,top=2cm,bottom=2cm,left=3cm,right=3cm,marginparwidth=1.75cm]{geometry}
\usepackage[colorlinks=true, allcolors=blue]{hyperref}

\title{DS Written Homework 1}
\author{Student ID: b10201054}

\begin{document}
\maketitle

\section*{Problem 1}
Let $f(n), T(n)$ be a real function and $\phi(n)$ be a positive function.

\begin{enumerate}
    \item [(a)] 
        Since $\lim_{n\to\infty}f(n)$ exists, there exists $c\in \mathbb{R}$ such that 
        \[
            \lim_{n\to\infty}f(n) = c
        \]
        If we want $\limsup_{n\to\infty}f(n) = c$, we need to show that for each $\epsilon > 0$, there exists $N_{\epsilon} \in \mathbb{N}$ such that
        \[
            \left\lvert c - \sup_{k\geq n}x_k \right\rvert  < \epsilon \text{ whenever } n \geq N_{\epsilon}
        \]
        By the definition of $\lim$, we have the following : for each $\epsilon > 0$, there exists $N_{\epsilon} \in \mathbb{N}$ such that
        \[
            \left\lvert c - x_n \right\rvert < \epsilon \text{ whenever } n \geq N_{\epsilon}
        \]
        Note that by the definition of $\sup$, for each $\epsilon > 0$, there exists $p_\epsilon \geq n$ such that
        \[
            \sup_{k \geq n}x_k - \epsilon < x_{p_\epsilon}
        \]
        Now if we choose $\epsilon_0 = \frac{\epsilon}{3} > 0$, there exists $N_{\epsilon_0}, p_{\epsilon_0} \in \mathbb{N}$ with $p_{\epsilon_0} \geq N_{\epsilon_0}$such that
        \[
            \left\lvert c - x_n \right\rvert < \epsilon_0 \text{ whenever } n \geq N_{\epsilon_0}
        \]
        \[
            \left\lvert x_{p_{\epsilon_0}} - x_n \right\rvert < \epsilon_0 \text{ whenever } n \geq N_{\epsilon_0}
        \]
        \[
            \left\lvert \sup_{k \geq n}x_k - x_{p_{\epsilon_0}}\right\rvert  < \epsilon_0
        \]
        Then we have
        \[
            \left\lvert c - \sup_{k\geq n}x_k \right\rvert \leq \left\lvert c - x_n \right\rvert + \left\lvert x_n - x_{p_{\epsilon_0}} \right\rvert + \left\lvert \sup_{k \geq n}x_k - x_{p_{\epsilon_0}}\right\rvert < \epsilon
        \]
        whenever $n \geq N_{\epsilon_0}$, which means $\limsup_{n\to\infty}f(n) = c$.

        Now prove $\liminf_{n\to\infty}f(n) = c$, we need to show that for each $\epsilon > 0$, there exists $N_{\epsilon} \in \mathbb{N}$ such that
        \[
            \left\lvert c - \inf_{k\geq n}x_k \right\rvert  < \epsilon \text{ whenever } n \geq N_{\epsilon}
        \]
        Note that by the definition of $\inf$, for each $\epsilon > 0$, there exists $p_\epsilon \geq n$ such that
        \[
            \inf_{k \geq n}x_k + \epsilon > x_{p_\epsilon}
        \]
        Similarly, if we choose $\epsilon_0 = \frac{\epsilon}{3} > 0$, there exists $N_{\epsilon_0}, p_{\epsilon_0} \in \mathbb{N}$ with $p_{\epsilon_0} \geq N_{\epsilon_0}$such that
        \[
            \left\lvert c - x_n \right\rvert < \epsilon_0 \text{ whenever } n \geq N_{\epsilon_0}
        \]
        \[
            \left\lvert x_{p_{\epsilon_0}} - x_n \right\rvert < \epsilon_0 \text{ whenever } n \geq N_{\epsilon_0}
        \]
        \[
            \left\lvert \inf_{k \geq n}x_k - x_{p_{\epsilon_0}}\right\rvert  < \epsilon_0
        \]
        Then we have
        \[
            \left\lvert c - \inf_{k\geq n}x_k \right\rvert \leq \left\lvert c - x_n \right\rvert + \left\lvert x_n - x_{p_{\epsilon_0}} \right\rvert + \left\lvert \inf_{k \geq n}x_k - x_{p_{\epsilon_0}}\right\rvert < \epsilon
        \]
        whenever $n \geq N_{\epsilon_0}$, which means $\liminf_{n\to\infty}f(n) = c$.
        Hence, we have the following result
        \[
            \lim_{n\to\infty} f(n) = \limsup_{n\to\infty} f(n) = \liminf_{n\to\infty} f(n) = c
        \]
    \item[(b)]
        $T(n) \in \Theta (\phi(n)) $ gives us both $T(n) \in O(\phi(n))$ and $T(n) \in \Omega(\phi(n))$, by the theorem taught in class, we have the following observations
        \[
            \limsup_{n\to\infty} \frac{\left\lvert T(n)\right\rvert }{\phi(n)} < \infty, \liminf_{n\to\infty} \frac{\left\lvert T(n)\right\rvert }{\phi(n)} > 0
        \]
        By the result given by (a), we have 
        \[
            \limsup_{n\to\infty} \frac{\left\lvert T(n)\right\rvert }{\phi(n)} = \liminf_{n\to\infty} \frac{\left\lvert T(n)\right\rvert }{\phi(n)} = \lim_{n\to\infty} \frac{\left\lvert T(n)\right\rvert }{\phi(n)}
        \]
        Then we have
        \[
            0 < \lim_{n\to\infty} \frac{\left\lvert T(n)\right\rvert }{\phi(n)} < \infty
        \]
    \item[(c)]
        Since $\lim_{n\to\infty} \frac{\left\lvert T(n)\right\rvert }{\phi(n)}$ exists, by the result given by (a), we have 
        \[
            \limsup_{n\to\infty} \frac{\left\lvert T(n)\right\rvert }{\phi(n)} = \liminf_{n\to\infty} \frac{\left\lvert T(n)\right\rvert }{\phi(n)} = \lim_{n\to\infty} \frac{\left\lvert T(n)\right\rvert }{\phi(n)}
        \]
        Then we have
        \[
            0 < \lim_{n\to\infty} \frac{\left\lvert T(n)\right\rvert }{\phi(n)} = \limsup_{n\to\infty} \frac{\left\lvert T(n)\right\rvert }{\phi(n)} = \liminf_{n\to\infty} \frac{\left\lvert T(n)\right\rvert }{\phi(n)} < \infty
        \]
        By the theorem taught in class, we have $T(n) \in O(\phi(n))$ and $T(n) \in \Omega (\phi(n))$.
        Hence $T(n) \in \Theta (\phi(n))$.
    \item[(d)]
        Consider the following condition
        \begin{equation}
            T(n) = \left\{
            \begin{aligned}
                2\phi(n) & \text{, if n is even} \\
                1\phi(n) & \text{, if n is odd}
            \end{aligned} 
            \right.
        \end{equation}
        Then we have $T(n) \in \Theta (\phi(n))$, but the limit $\lim_{n\to\infty} \frac{\left\lvert T(n)\right\rvert }{\phi(n)}$ does not exist.
        This is the counterexample.
\end{enumerate}

\section*{Problem 2}    
Assume $f(n), g(n), h(n)$ are all positive function.
\begin{enumerate}
    \item[(a)]
        $f(n)\in O(g(n))$ and $g(n)\in O(h(n))$ gives us $f(n)\leq c_{1}g(n), g(n) \leq c_{2}h(n)$. Hence we have
        \[
            f(n) \leq c_{1}g(n) \leq c_{1}c_{2}h(n) \leq ch(n)
        \]
        This gives us $f(n)\in O(h(n))$
    \item[(b)]
        $f(n)\in O(g(n))$ means $f(n)\leq c_{1}g(n)$. Since $f(n), g(n)$ are positive, we have $c_{1}$ also be positive. Hence we have
        \[
            g(n) \geq \frac{1}{c_{1}} f(n)
        \]
        This gives us $g(n)\in \Omega (f(n))$
    \item[(c)]
        $f(n)\in \omega(g(n))$ means for all constants $c>0$, there exists an $n_0$ such that $f(n)>cg(n)$ when $n\geq n_0$.
        
        Then we have for all constants $c>0$, there exists an $n_0$ such that $g(n)<\frac{1}{c}f(n)$ when $n\geq n_0$. This gives us $g(n)\in o(f(n))$.
    \item[(d)]
        Consider the following $g(n)$
        \begin{equation}
            g(n) = \left\{
            \begin{aligned}
                nf(n) & \text{, if n is even} \\
                \frac{f(n)}{n} & \text{, otherwise}
            \end{aligned} 
            \right.
        \end{equation}
        By the definition of big-O notations, if either $f(n)\in O(g(n))$ or $g(n)\in O(f(n))$, we need to find a constant $c>0$ and $N$ such that either $f(n)\leq cg(n)$ or $g(n)\leq cf(n)$ must be satisfied.
        In this case, we cannot find any constant $c>0$ which is independent of n to satisfy the inequations.

        Hence, "Either $f(n)\in O(g(n))$ or $g(n)\in O(f(n))$ is true." is false.
\end{enumerate}

\section*{Problem 3}    

\begin{enumerate}
    \item[(a)] 
        Here we use limit supremum to prove. 
        \[
            \limsup_{n\to\infty} \frac{2^{2n}}{2^{2n+1024}}=\limsup_{n\to\infty} \frac{1}{2^{1024}} = \frac{1}{2^{1024}} < \infty
        \]
        Hence $2^{2n}\in O(2^{2n+1024})$
    \item[(b)]
        Note that $\log_{1024}n^{2} = 2 \log_{1024} n = 2\frac{\log n}{\log 1024}, \log_{2}n^{1024} = 1024 \log_{2} n = 1024 \frac{\log n}{\log 2}$
        Then we have
        \[
            \limsup_{n\to\infty} \frac{\log_{1024}n^{2}}{\log_{2}n^{1024}} = \limsup_{n\to\infty} \frac{\frac{2\log n}{\log 1024}}{\frac{1024\log n}{\log 2}} = \limsup_{n\to\infty} \frac{2 \log 2}{1024 \log 1024} = \frac{1}{5120} \neq 0
        \]
        Hence $\log_{1024} n^{2} \notin o(\log_{2} n^{1024})$
    \item[(c)]
        From the Stirling's approximation, we have $n!\sim \sqrt{2\pi n}\left(\frac{n}{e}\right)^{n}$ when $n$ is large enough.
        Then we get 
        \[
            \log(n!) \sim \log\left(\sqrt{2\pi n}\left(\frac{n}{e}\right)^{n}\right) = n(\log n - \log e) + 0.5(\log {n} + \log 2\pi)
        \]
        \[
            \frac{\log(n!)}{n\log n} = 1 - \frac{\log e}{\log n} + \frac{1}{2n} + \frac{\log 2\pi}{2n\log n}
        \]
        Hence, we have $\lim_{n\to\infty} \frac{\log(n!)}{n\log n} = 1$.
        By the result of 1.(c), we have $$\log(n!) \in \Theta(n\log n)$$
    \item[(d)]
        $x^{2.5} = \left\lfloor x^{2.5}\right\rfloor + \left\{ x^{2.5}\right\} $, where $\left\{ x^{2.5}\right\} $ is the fraction part of $x^{2.5}$.
        Then we have
        \[
            \lim_{x\to\infty} \frac{\left\lfloor x^{2.5}\right\rfloor}{x^{2.5}} = \lim_{x\to\infty} \frac{x^{2.5} - \left\{ x^{2.5}\right\}}{x^{2.5}} = 1
        \]
        By the result of 1.(c), we have $\left\lfloor x^{2.5}\right\rfloor \in \Theta(x^{2.5})\Rightarrow \left\lfloor x^{2.5}\right\rfloor \in \Omega(x^{2.5})$
    \item[(e)]
        $\left\lceil \frac{x}{2}\right\rceil = \frac{x}{2} + 1 - \left\{ \frac{x}{2}\right\}$, where $\left\{ \frac{x}{2}\right\} $ is the fraction part of $\frac{x}{2}$.
        \[
            \frac{x\left\lceil \frac{x}{2}\right\rceil}{x^2} = \frac{x(\frac{x}{2} + 1 - \left\{ \frac{x}{2}\right\})}{x^2} = \frac{1}{2} + \frac{1}{x} - \frac{\left\{ \frac{x}{2}\right\}}{x}
        \]
        Then we have
        \[
            x\left\lceil \frac{x}{2}\right\rceil = 2x^2 + \left(1-\left\{\frac{x}{2}\right\} \right)x
        \]
        When $x>1$, we know that $x < x^2$, hence the $\left(1-\left\{\frac{x}{2}\right\} \right)x$ part has the upperbound $x^2$.
        So that we finally get the result
        \[
            x\left\lceil \frac{x}{2}\right\rceil \leq 3x^2 
        \]
        for $x>1$.
        This gives us $x\left\lceil \frac{x}{2}\right\rceil \in O(x^2)$
\end{enumerate}

\section*{Problem 4}

\[
    f_{10}(n) \succ f_{9}(n) \succ f_{4}(n) \succ f_{12}(n) \succ f_{2}(n) \succ f_{3}(n)    
\]
\[
    f_{3}(n) \sim f_{13}(n) \succ f_{1}(n) \succ f_{5}(n) \succ f_{11}(n) \succ f_{7}(n) \succ f_{6}(n)
\]
\\
$f_{10} \succ f_{9}$:
\[
    \lim_{n\to\infty} \frac{\log\log n}{10^{10^10}} = \infty
\]
\\
$f_{9} \succ f_{4}$:
\[
    \lim_{n\to\infty} \frac{\sqrt{\log n}}{\log\log n} = \lim_{n\to\infty} \frac{\frac{1}{2x\sqrt{\log x}}}{\frac{1}{x\log x}} = \lim_{n\to\infty} \frac{\sqrt{\log x}}{2} = \infty
\]
\\
$f_{4} \succ f_{12}$:
\[
    \lim_{n\to\infty} \frac{(\log n)^{1.5}}{\sqrt{\log n}} = \lim_{n\to\infty} \log n = \infty
\]
\\
$f_{12} \succ f_{2}$:
\[
    10^{\log n^2} = (e^{\log10})^{2\log n} = (e^{\log n})^{2\log 10}= n^{2\log 10}
\]
\[
    \lim_{n\to\infty} \frac{n^{2\log 10}}{(\log n)^{1.5}} = \lim_{n\to\infty} \frac{(2\log 10) n^{(2\log 10) - 1}}{\frac{1.5(\log n)^{0.5}}{n}} = \lim_{n\to\infty} \frac{(2\log 10) n^{2\log 10}}{1.5(\log n)^{0.5}} = \infty
\]
\\
$f_{2} \succ f_{3}$:
\[
    \lim_{n\to\infty} \frac{n^6}{n^{2\log 10}} = \infty \text{ since } 6 > 2\log 10
\]
\\
$f_{3} \sim f_{13}$:
\[
    \sum_{k = 1}^{n} k^5 = \frac{1}{12} n^2 (n + 1)^2 (2n^2 + 2n - 1) = \frac{1}{6} n^6 + \frac{1}{2} n^5 + \frac{5}{12} n^4 - \frac{1}{12} n^2
\]
\[
    \lim_{n\to\infty} \frac{\sum_{k = 1}^{n} k^5}{n^6} = \frac{1}{6}
\]
\\
$f_{13} \succ f_{8}$:
Suppose d is a constant, we have
\[
    d \log n < (\log \log n) (\log n) \Rightarrow n^{d} < n^{\log\log n}
\]
\[
    \lim_{n\to\infty} \frac{n^{\log\log n}}{\sum_{k = 1}^{n} k^5} = \lim_{n\to\infty} \frac{n^{\log\log n}}{\frac{1}{6} n^5 + \frac{1}{2} n^4 + \frac{5}{12} n^3 - \frac{1}{12} n} = \infty
\]
\\
$f_{8} \succ f_{1}$:
\[
    (\log \log n) (\log n) < \log n \log n < n < n \log \frac{3}{2} \Rightarrow n^{\log\log n} < (\frac{3}{2})^n
\]
\[
    \lim_{n\to\infty} \frac{n(\frac{3}{2})^n}{n^{\log\log n}} = \infty
\]
\\
$f_{1} \succ f_{5}$:
\[
    \lim_{n\to\infty} \frac{3^n}{n(\frac{3}{2})^n} = \lim_{n\to\infty} \frac{2^n}{n} = \infty
\]
\\
$f_{5} \succ f_{11}$
\[
    \lim_{n\to\infty} \frac{n!}{3^n} = \lim_{n\to\infty} \frac{\sqrt{2\pi n}\left(\frac{n}{e}\right)^{n}}{3^n} = \lim_{n\to\infty}  \sqrt{2\pi n}\left(\frac{n}{3e}\right)^{n} = \infty
\]
\\
$f_{11} \succ f_{7}$
\[
    \lim_{n\to\infty} \frac{n^n}{n!} = \lim_{n\to\infty} \frac{n^n}{\sqrt{2\pi n}\left(\frac{n}{e}\right)^{n}} = \lim_{n\to\infty} \frac{e^{n}}{\sqrt{2\pi n}} = \infty
\]
\\
$f_{7} \succ f_{6}$
\[
    6^{n} \log 6 > n \log n \Rightarrow 6^{6^n} > n^{n} 
\]

\section*{Problem 5}

\begin{enumerate}
    \item[(a)] 
        Suppose $c_1, c_2$ are two constants such that $f(n)\leq c_1h(n), g(n)\leq c_2h(n)$, then we have
        \[
            f(n) + g(n) \leq (c_1 + c_2)h(n) = ch(n)
        \]
        Hence, $f(n) + g(n) \in O(h(n))$
    \item[(b)]
        Since $f, g$ are positive, we have $\left\lvert f(n) - g(n) \right\rvert \leq \max(f(n), g(n))$. Then either $\left\lvert f(n) - g(n) \right\rvert \in O(f(n))$ or $\left\lvert f(n) - g(n) \right\rvert \in O(g(n))$ would be satisfied.
        This results that $\left\lvert f(n) - g(n) \right\rvert \in O(h(n))$ because $f(n), g(n) \in O(h(n))$
    \item[(c)]
        Since $f, g$ are positive, suppose $c_1$ is a constant that $f(n)\leq c_1g(n)$. Square both sides of the inequation, we have $(f(n))^2 \leq (c_1)^2(g(n))^2$.
        Hence, $(f(n))^2 \in O((g(n))^2)$
    \item[(d)]
        Counterexample: $f(n) = n, g(n) = \frac{n}{2}$, then we have $2^{f(n)} = 2^{n}, 2^{g(n)} = (\sqrt{2})^{n}$.
        \[
            \lim_{n\to\infty} \frac{2^{n}}{(\sqrt{2})^n} = \lim_{n\to\infty} (\sqrt{2})^n = \infty
        \]
        Hence, $2^{f(n)} \notin O(2^{g(n)})$
    \item[(e)] 
        Counterexample: Suppose $f(n) = \log n, g(n) = n, h(n) = n^{2}$, we have $f(g(n)) = \log n, f(h(n)) = 2\log n$. Then $f(g(n)) \notin o(f(h(n)))$. 
\end{enumerate}

\section*{Problem 6}

\begin{enumerate}
    \item[(a)]
        The loop from line 4 to line 7 runs $n$ times, and for each loop, the line 6 runs $k$ times. 
        Hence the time complexity is 
        \[
            \sum_{k=1}^{n} k\Theta(1) = \Theta(n^2)
        \]
    \item[(b)] 
        The loop from line 4 to line 7 runs $n$ times, and for each loop, the line 6 runs $k$ times.
        When the line 6 runs the first time of the loop, the time complexity is $\Theta(\min(x, k)) = \Theta(1)$.
        After the first time of the loop, the time complexity is $\Theta(\min(x, k)) = \Theta(k)$
        Sum up the complexity and we have the total time complexity of the $k_{th}$ loop be $(k-1)\Theta(k) + \Theta(1) = \Theta(k^2)$.
        Now compute $n$ times, we get the time complexity
        \[
            \sum_{k=1}^{n} \Theta(k^2) = \Theta(k^3)
        \]
\end{enumerate}

\end{document}
